hardware/ag32MachineScript.sml
@@ -59,7 +59,7 @@ val _ = Datatype `
           (*data_in : word32;*)
 
           (* Memory *)
-          mem : word32 -> word32;
+          mem : word32 -> word8;
           error : word2;
           ready : bool;
           data_rdata : word32;
@@ -72,23 +72,17 @@ val _ = Datatype `
           (* Interrupt *)
           interrupt_state : interrupt_state;
           interrupt_ack : bool;
-          io_events : (word32 -> word32) list
+          io_events : (word32 -> word8) list
         |>`;
 
 (** Memory specification **)
 
 val mem_update_def = Define `
  mem_update mem addr wdata wstrb =
-  let
-    oldv = mem addr;
-    newv = (case wstrb of
-       1w  (* 0001 *) => bit_field_insert 7 0 ((7 >< 0) wdata) oldv
-     | 2w  (* 0010 *) => bit_field_insert 15 8 ((15 >< 8) wdata) oldv
-     | 4w  (* 0100 *) => bit_field_insert 23 16 ((23 >< 16) wdata) oldv
-     | 8w  (* 1000 *) => bit_field_insert 31 24 ((31 >< 24) wdata) oldv
-     | 15w (* 1111 *) => wdata)
-  in
-    (addr =+ newv) mem`;
+  let mem = if word_bit 0 wstrb then (addr      =+ ((7 >< 0) wdata)) mem else mem;
+      mem = if word_bit 1 wstrb then (addr + 1w =+ ((15 >< 8) wdata)) mem else mem;
+      mem = if word_bit 2 wstrb then (addr + 2w =+ ((23 >< 16) wdata)) mem else mem in
+            if word_bit 3 wstrb then (addr + 3w =+ ((31 >< 24) wdata)) mem else mem`;
 
 (* TODO: Consider using alignmentTheory instead *)
 val align_addr_def = Define `
@@ -116,7 +110,12 @@ val fext_accessor_circuit_def = Define `
 
      get_interrupt_req := state_circuit_interrupt_req |>`;
 
+val word_at_addr_def = Define `
+ word_at_addr (mem : word32 -> word8) addr =
+  (mem (addr + 3w) @@ (mem (addr + 2w) @@ (mem (addr + 1w) @@ mem addr):word16):word24):word32`;
+
 (* TODO: Should maybe add that errors are not allowed to occur, i.e. non-error implies this ... *)
+(* TODO: Would make more sense to have alignment preconds, rather than doing alignment "automatically" *)
 val is_mem_def = Define `
  is_mem accessors step fext =
   !n.
@@ -131,31 +130,31 @@ val is_mem_def = Define `
   (accessors.get_command (step n) = 1w /\ (fext n).ready ==>
    ?m. (!p. p < m ==> (fext (SUC (n + p))).mem = (fext n).mem /\ ~(fext (SUC (n + p))).ready) /\
        (fext (SUC (n + m))).mem = (fext n).mem /\
-       (fext (SUC (n + m))).inst_rdata = (fext n).mem (align_addr (accessors.get_PC (step n))) /\
+       (fext (SUC (n + m))).inst_rdata = word_at_addr (fext n).mem (align_addr (accessors.get_PC (step n))) /\
        (fext (SUC (n + m))).ready) /\
 
   (* Read instruction + read data *)
   (accessors.get_command (step n) = 2w /\ (fext n).ready ==>
     ?m. (!p. p < m ==> (fext (SUC (n + p))).mem = (fext n).mem /\ ~(fext (SUC (n + p))).ready) /\
         (fext (SUC (n + m))).mem = (fext n).mem /\
-        (fext (SUC (n + m))).data_rdata = (fext n).mem (accessors.get_data_addr (step n)) /\
-        (fext (SUC (n + m))).inst_rdata = (fext n).mem (align_addr (accessors.get_PC (step n))) /\
+        (fext (SUC (n + m))).data_rdata = word_at_addr (fext n).mem (align_addr (accessors.get_data_addr (step n))) /\
+        (fext (SUC (n + m))).inst_rdata = word_at_addr (fext n).mem (align_addr (accessors.get_PC (step n))) /\
         (fext (SUC (n + m))).ready) /\
 
   (* Read instruction + write data, note that the current unverified cache layer do not allow inst read addr and
                                     data write addr to be the same... *)
   (accessors.get_command (step n) = 3w /\ (fext n).ready ==>
     ?m. (!p. p < m ==> (fext (SUC (n + p))).mem = (fext n).mem /\ ~(fext (SUC (n + p))).ready) /\
-        (let newmem = mem_update (fext n).mem (accessors.get_data_addr (step n)) (accessors.get_data_wdata (step n)) (accessors.get_data_wstrb (step n)) in
+        (let newmem = mem_update (fext n).mem (align_addr (accessors.get_data_addr (step n))) (accessors.get_data_wdata (step n)) (accessors.get_data_wstrb (step n)) in
          (fext (SUC (n + m))).mem = newmem /\
-         (fext (SUC (n + m))).inst_rdata = newmem (align_addr (accessors.get_PC (step n))) /\
+         (fext (SUC (n + m))).inst_rdata = word_at_addr newmem (align_addr (accessors.get_PC (step n))) /\
          (fext (SUC (n + m))).ready)) /\
 
  (* Clear cache block used for printing ... exactly the same semantics as "read instruction" *)
  (accessors.get_command (step n) = 4w /\ (fext n).ready ==>
    ?m. (!p. p < m ==> (fext (SUC (n + p))).mem = (fext n).mem /\ ~(fext (SUC (n + p))).ready) /\
        (fext (SUC (n + m))).mem = (fext n).mem /\
-       (fext (SUC (n + m))).inst_rdata = (fext n).mem (align_addr (accessors.get_PC (step n))) /\
+       (fext (SUC (n + m))).inst_rdata = word_at_addr (fext n).mem (align_addr (accessors.get_PC (step n))) /\
        (fext (SUC (n + m))).ready)`;
 
 (** Accelerator specification **)
@@ -279,12 +278,12 @@ val execute_instruction_def = Define `
 
     (* StoreMEM *)
   | 2w => s with <|state := 1w; command := 3w; PC := PC_next;
-                   data_addr := align_addr bV; data_wdata := aV; data_wstrb := 15w|>
+                   data_addr := bV; data_wdata := aV; data_wstrb := 15w|>
 
     (* StoreMEMByte *)
     (* TODO: Can reuse shifter here? *)
   | 3w => (let s = s with <|state := 1w; command := 3w; PC := PC_next;
-                            data_addr := align_addr bV; data_wstrb := 1w <<~ w2w ((1 >< 0) bV)|> in
+                            data_addr := bV; data_wstrb := 1w <<~ w2w ((1 >< 0) bV)|> in
              (case (1 >< 0) bV of
                0w => s with data_wdata := bit_field_insert 7 0 ((7 >< 0) aV) s.data_wdata
              | 1w => s with data_wdata := bit_field_insert 15 8 ((7 >< 0) aV) s.data_wdata
@@ -293,11 +292,11 @@ val execute_instruction_def = Define `
 
     (* LoadMEM *)
   | 4w => s with <|state := 1w; command := 2w; PC := PC_next;
-                   data_addr := align_addr aV; do_delay_write := 4w; delay_write := (30 >< 25) s.i|>
+                   data_addr := aV; do_delay_write := 4w; delay_write := (30 >< 25) s.i|>
 
     (* LoadMEMByte *)
   | 5w => s with <|state := 1w; command := 2w; PC := PC_next;
-                   data_addr := align_addr aV; do_delay_write := w2w ((1 >< 0) aV);
+                   data_addr := aV; do_delay_write := w2w ((1 >< 0) aV);
                    delay_write := (30 >< 25) s.i|>
 
     (* Out *)
